compiler/src/compiler/RecurseWithFun.v
@@ -8,7 +8,8 @@ Hypothesis Rwf : well_founded R.
 Variable P : Type. (* really I want to say that P gives one type for each equivalence class
                       of A wrt the equivalence relation E.  Not clear how to say this though.*)
 Variable F : forall x:A, (forall y:A, R y x -> P) -> P.
-Variable E : A -> A -> Prop.
+Variable E1 : A -> A -> Prop.
+Variable E2 : P -> P -> Prop.
 
 Fixpoint my_Fix_F (x:A) (a:Acc R x) : P :=
   F x (fun (y:A) (h:R y x) => my_Fix_F y (Acc_inv a h)).
@@ -29,12 +30,12 @@ Definition my_Fix (x:A) := my_Fix_F x (Rwf x).
 Hypothesis
   F_ext :
   forall (x1 x2:A) (f1:forall y:A, R y x1 -> P) (f2:forall y:A, R y x2 -> P),
-    E x1 x2 ->
+    E1 x1 x2 ->
     (forall (y1 y2:A) (p1:R y1 x1) (p2:R y2 x2),
-        E y1 y2 -> f1 y1 p1 = f2 y2 p2) -> F x1 f1 = F x2 f2.
+        E1 y1 y2 -> E2 (f1 y1 p1) (f2 y2 p2)) -> E2 (F x1 f1) (F x2 f2).
 
 Lemma my_Fix_F_inv : forall (x1 x2:A) (r1:Acc R x1) (r2:Acc R x2),
-    E x1 x2 -> my_Fix_F x1 r1 = my_Fix_F x2 r2.
+    E1 x1 x2 -> E2 (my_Fix_F x1 r1) (my_Fix_F x2 r2).
 Proof.
   intro x1; induction (Rwf x1); intros x2 r1 r2.
   rewrite <- (my_Fix_F_eq x r1); rewrite <- (my_Fix_F_eq x2 r2); intros.
@@ -42,7 +43,7 @@ Proof.
 Qed.
 
 Lemma my_Fix_eq : forall (x1 x2:A),
-    E x1 x2 -> my_Fix x1 = F x2 (fun (y:A) (p:R y x2) => my_Fix y).
+    E1 x1 x2 -> E2 (my_Fix x1) (F x2 (fun (y:A) (p:R y x2) => my_Fix y)).
 Proof.
   intro x; unfold my_Fix.
   rewrite <- my_Fix_F_eq.
